Work on transitivity proof - mostly in interpolation_II.

sepcomp-reserved/mem_interpolation_defs.v
@@ -28,6 +28,7 @@ destruct pp; simpl in *. exfalso. apply H. apply perm_any_N.
 trivial.
 Qed.
 
+(*
 Definition isSource j m1 (b2:block) (ofs2:Z) b : option Z :=
   match j b with None => None
          | Some (bb,delta) => if eq_block b2 bb 
@@ -207,6 +208,351 @@ Proof. intros. intros b1; intros.
      apply VALIDBLOCK. apply (Mem.valid_block_inject_1 _ _ _ _ _ _ H Inj12).
      apply H.
 Qed.
+*)
+
+Definition isSourceP (P: block -> Z -> Prop) (pdec: forall b ofs, {P b ofs} + {~ P b ofs})
+                j (b2:block) (ofs2:Z) b : option Z :=
+  match j b with None => None
+         | Some (bb,delta) => if eq_block b2 bb 
+                                             then if pdec b (ofs2 - delta) 
+                                                     then Some (ofs2 - delta)  else None
+                                             else None
+  end.
+
+Lemma isSourceP_NoneE: forall P pdec j b2 ofs2 b1, None = isSourceP P pdec j b2 ofs2 b1 ->
+    j b1 = None \/ (exists b, exists delta, j b1 = Some (b,delta) /\ b<>b2) \/
+    (exists delta, j b1 = Some(b2,delta) /\ ~P b1 (ofs2-delta)).
+Proof. intros. unfold isSourceP in H.
+  remember (j b1) as zz.
+  destruct zz. destruct p.
+     destruct (eq_block b2 z). subst.
+       remember (pdec b1 (ofs2 - z0)) as d.
+       destruct d; inv H. right. right. exists z0. split; trivial. 
+     right. left. exists z. exists z0. split; auto. 
+  left; trivial. 
+Qed.
+
+Lemma isSourceP_SomeE: forall P pdec j b2 ofs2 b1 ofs1, Some ofs1 = isSourceP P pdec j b2 ofs2 b1 ->
+    exists delta, j b1 = Some(b2,delta) /\ P b1 ofs1 /\ ofs2=ofs1+delta.
+Proof. intros. unfold isSourceP in H.
+  remember (j b1) as zz.
+  destruct zz. destruct p.
+     destruct (eq_block b2 z). subst.
+       remember (pdec b1 (ofs2 - z0)) as d.
+       destruct d; inv H. exists z0. split; trivial. split; trivial. omega.
+    inv H.
+  inv H.
+Qed.
+
+Lemma isSourceP_SomeI: forall (P: block -> Z -> Prop) pdec j b2 ofs2 b1 delta, 
+       j b1 = Some(b2,delta) -> P b1 (ofs2 - delta) ->
+        isSourceP P pdec j b2 ofs2 b1 = Some (ofs2-delta).
+Proof. intros. unfold isSourceP. rewrite H.
+     destruct (eq_block b2 b2). subst.
+       remember (pdec b1 (ofs2 - delta)) as d.
+       destruct d. trivial.  exfalso. apply (n H0).
+     exfalso. apply n. trivial.
+Qed.
+
+Lemma isSourceP_SomeI': forall (P:block -> Z -> Prop) pdec j b2 ofs1 b1 delta, 
+       j b1 = Some(b2,delta) -> P b1 ofs1 ->
+        isSourceP P pdec j b2 (ofs1+delta) b1 = Some ofs1.
+Proof. intros. unfold isSourceP. rewrite H.
+     destruct (eq_block b2 b2). subst.
+       assert (ofs1 = ofs1 + delta - delta). omega. rewrite <- H1.
+       remember (pdec b1 ofs1) as d.
+       destruct d. trivial.  exfalso. apply (n H0).
+     exfalso. apply n. trivial.
+Qed.
+
+Fixpoint sourcePN P pdec (n:nat) j (b2:block) (ofs2:Z): option(block * Z) :=
+  match isSourceP P pdec j b2 ofs2 (Z_of_nat n) with 
+         Some ofs1 => Some (Z_of_nat n, ofs1)
+       | None => match n with O => None | S k => sourcePN P pdec k j b2 ofs2 end
+  end.
+
+Lemma sourcePN_SomeE: forall P pdec n j b2 ofs2 b1 ofs1, 
+    sourcePN P pdec n j b2 ofs2 = Some(b1,ofs1) ->
+    exists delta, 0 <= b1 <= (Z_of_nat n) /\ j b1 = Some(b2,delta) /\ 
+                  P b1 ofs1 /\ ofs2=ofs1+delta.
+Proof. intros P pdec n.
+  induction n; simpl; intros.
+     remember (isSourceP P pdec j b2 ofs2 0) as d.
+     destruct d; inv H.  
+           apply isSourceP_SomeE in Heqd. destruct Heqd as [delta [J [PP Off]]]. 
+           exists delta; repeat split; auto; omega. 
+  remember (isSourceP P pdec j b2 ofs2 (Zpos (P_of_succ_nat n)) ) as d.
+  destruct d. inv H. clear IHn.
+           apply isSourceP_SomeE in Heqd. destruct Heqd as [delta [J [PP Off]]]. 
+           exists delta; repeat split; auto. apply Zle_0_pos. omega.
+   apply IHn in H. destruct H as [delta [Bounds [J [PP Off]]]]. 
+       exists delta; repeat split; auto. omega.
+       eapply Zle_trans. apply Bounds. rewrite Zpos_P_of_succ_nat. omega. 
+Qed.
+
+Lemma sourcePN_NoneE: forall P pdec n j b2 ofs2, 
+    sourcePN P pdec n j b2 ofs2 = None -> 
+    forall b1 delta, 0 <= b1 <= (Z_of_nat n) -> j b1 = Some(b2,delta) ->
+                     ~ P b1 (ofs2-delta).
+Proof. intros P pdec n.
+  induction n; simpl; intros. assert (b1=0). omega. subst. clear H0.
+     remember (isSourceP P pdec j b2 ofs2 0) as d.
+     destruct d; inv H.  
+           apply isSourceP_NoneE in Heqd. destruct Heqd. congruence. 
+           destruct H. destruct H as [b [delta1 [J PP]]]. 
+                rewrite J in H1. inv H1. exfalso. apply PP. trivial. 
+           destruct H as [ddelta [J PP]]. rewrite J in H1. inv H1. assumption. 
+  remember (isSourceP P pdec j b2 ofs2 (Zpos (P_of_succ_nat n)) ) as d.
+  destruct d. inv H. specialize (IHn _ _ _ H).
+           destruct H0. rewrite Zpos_P_of_succ_nat in H2. apply Z_le_lt_eq_dec in H2. 
+           destruct H2. assert (0 <= b1 <= Z_of_nat n). omega. 
+               apply (IHn _ _ H2 H1). 
+           subst.  
+           apply isSourceP_NoneE in Heqd.
+           destruct Heqd.
+           (*1/3*) rewrite Zpos_P_of_succ_nat in H2.  rewrite H1 in H2. inv H2. 
+           destruct H2. 
+            (*2/3*) destruct H2 as [b [d [J NEQ]]]. rewrite Zpos_P_of_succ_nat in J. 
+                    rewrite H1 in J. inv J. exfalso. apply NEQ. trivial. 
+           (*3.3*) destruct H2 as [d [J NP]]. rewrite Zpos_P_of_succ_nat in *. 
+                    rewrite H1 in J. inv J. apply NP. 
+Qed.
+
+Lemma sourcePN_SomeI: forall (P: block -> Z -> Prop) pdec n j m b2 b1 
+   ofs1 delta (OV:Mem.meminj_no_overlap j m),
+   j b1 = Some(b2,delta) -> P b1 ofs1 ->
+   (0 <= b1 <= Z_of_nat n) ->
+   forall (HH: forall b ofs, P b ofs -> Mem.perm m b ofs Max Nonempty),
+   sourcePN P pdec n j b2 (ofs1+delta) = Some(b1,ofs1).
+Proof. intros. 
+  remember (sourcePN P pdec n j b2 (ofs1 + delta)) as src.
+  destruct src; apply eq_sym in Heqsrc. 
+  Focus 2. assert (ZZ:= sourcePN_NoneE _ _ _ _ _ _ Heqsrc _ _ H1 H).
+           exfalso. assert (ofs1 + delta - delta = ofs1). omega.
+                    rewrite H2 in ZZ. apply (ZZ H0).
+  (*Some*) destruct p as [b off].
+       apply sourcePN_SomeE in Heqsrc.
+       destruct Heqsrc as [d [Hd [J [PP X]]]].
+       destruct (eq_block b1 b).
+          subst. rewrite H in J. inv J.
+          assert (ofs1 = off). omega. subst. trivial.
+       apply HH in H0. apply HH in PP.
+       destruct (OV _ _ _ _ _ _ _ _ n0 H J H0 PP).
+          exfalso. apply H2; trivial.
+       rewrite X in H2. exfalso. apply H2. trivial.
+Qed.  
+
+Definition  sourceP P pdec j m (b2:block) (ofs2:Z) : option(block * Z) :=
+   sourcePN P pdec (Zabs_nat ((Mem.nextblock m) - 1)) j b2 ofs2.
+
+Lemma sourceP_SomeE: forall P pdec j m (b2:block) (ofs2:Z) p, 
+  Some p = sourceP P pdec j m b2 ofs2 -> 
+    exists b1, exists delta, exists ofs1, 
+                  p = (b1,ofs1) /\
+                  0 <= b1 < Mem.nextblock m /\ j b1 = Some(b2,delta) /\ 
+                  P b1 ofs1 /\ ofs2=ofs1+delta.
+Proof. intros. unfold sourceP in H.
+  destruct p as [b1 ofs1]; subst. apply eq_sym in H.      
+  apply sourcePN_SomeE in H. 
+  destruct H as [delta [Bounds [J [PP Off]]]]; subst. 
+  exists b1; exists delta; exists ofs1. split; trivial. 
+  split. rewrite inj_Zabs_nat in Bounds. 
+         destruct Bounds; split; trivial. 
+         assert (NB:= Mem.nextblock_pos m).
+         destruct (Zabs_spec (Mem.nextblock m - 1)).
+           destruct H1.  rewrite H2 in H0. omega.
+         destruct H1. exfalso. omega.
+  repeat split; auto.
+Qed.
+  
+Lemma sourceP_NoneE: forall P pdec j m b2 ofs2, 
+    None = sourceP P pdec j m b2 ofs2 -> 
+    forall b1 delta, 0 <= b1 < Mem.nextblock m -> j b1 = Some(b2,delta) ->
+                     ~P b1 (ofs2-delta). 
+Proof. intros. apply eq_sym in H. unfold sourceP in H.    
+  eapply (sourcePN_NoneE _ _ _ _ _ _ H b1 delta); trivial. 
+  clear H H1. rewrite inj_Zabs_nat.
+  split. apply H0.
+  destruct (Zabs_spec (Mem.nextblock m - 1)); destruct H; rewrite H1; omega. 
+Qed.  
+
+Lemma sourceP_SomeI: forall (P: block -> Z -> Prop) pdec j m b2 b1 
+   ofs1 delta (OV:Mem.meminj_no_overlap j m),
+   j b1 = Some(b2,delta) -> P b1 ofs1 ->
+   forall (HH: forall b ofs, P b ofs -> Mem.perm m b ofs Max Nonempty),
+   sourceP P pdec j m b2 (ofs1+delta) = Some(b1,ofs1).
+Proof. intros. unfold sourceP.
+  eapply sourcePN_SomeI; try eassumption.
+  apply HH in H0.
+  destruct (VALIDBLOCK _ _ (Mem.perm_valid_block _ _ _ _ _ H0)). 
+  clear H OV. rewrite inj_Zabs_nat.
+  destruct (Zabs_spec (Mem.nextblock m - 1)); destruct H; rewrite H3; omega.
+Qed.
+
+(*some equivalent will be needed
+Lemma sourcePNone_LOOR: forall j m1 b2 ofs2 (N: None = sourceP j m1 b2 ofs2) m2
+              (Inj12: Mem.inject j m1 m2), loc_out_of_reach j m1 b2 ofs2.
+Proof. intros. intros b1; intros.
+   eapply sourceP_NoneE.
+     apply N. 
+     apply VALIDBLOCK. apply (Mem.valid_block_inject_1 _ _ _ _ _ _ H Inj12).
+     apply H.
+Qed.
+*)
+
+Definition isSource j m1 := 
+isSourceP (fun b ofs => Mem.perm m1 b ofs Max Nonempty)
+          (fun b ofs => Mem.perm_dec m1 b ofs Max Nonempty) j.
+
+Lemma isSource_NoneE: forall j m b2 ofs2 b1, None = isSource j m b2 ofs2 b1 ->
+    j b1 = None \/ (exists b, exists delta, j b1 = Some (b,delta) /\ b<>b2) \/
+    (exists delta, j b1 = Some(b2,delta) /\ ~ Mem.perm m b1 (ofs2-delta) Max Nonempty).
+Proof. intros. 
+  apply (isSourceP_NoneE
+          (fun b ofs => Mem.perm m b ofs Max Nonempty)
+          (fun b ofs => Mem.perm_dec m b ofs Max Nonempty)).
+  auto. 
+Qed.
+
+Lemma isSource_SomeE: forall j m b2 ofs2 b1 ofs1, Some ofs1 = isSource j m b2 ofs2 b1 ->
+    exists delta, j b1 = Some(b2,delta) /\ Mem.perm m b1 ofs1 Max Nonempty /\ ofs2=ofs1+delta.
+Proof. intros. 
+  apply (isSourceP_SomeE
+          (fun b ofs => Mem.perm m b ofs Max Nonempty)
+          (fun b ofs => Mem.perm_dec m b ofs Max Nonempty)).
+  auto. 
+Qed.
+
+Lemma isSource_SomeI: forall j m b2 ofs2 b1 delta, 
+       j b1 = Some(b2,delta) -> Mem.perm m b1 (ofs2 - delta) Max Nonempty ->
+        isSource j m b2 ofs2 b1 = Some (ofs2-delta).
+Proof. intros.
+  apply (isSourceP_SomeI
+          (fun b ofs => Mem.perm m b ofs Max Nonempty)
+          (fun b ofs => Mem.perm_dec m b ofs Max Nonempty));
+  auto. 
+Qed. 
+
+Lemma isSource_SomeI': forall j m b2 ofs1 b1 delta, 
+       j b1 = Some(b2,delta) -> Mem.perm m b1 ofs1 Max Nonempty ->
+        isSource j m b2 (ofs1+delta) b1 = Some ofs1.
+Proof. intros. 
+  apply (isSourceP_SomeI'
+          (fun b ofs => Mem.perm m b ofs Max Nonempty)
+          (fun b ofs => Mem.perm_dec m b ofs Max Nonempty));
+  auto. 
+Qed. 
+
+Definition sourceN  (n:nat)  j m (b2:block) (ofs2:Z): option(block * Z) :=
+  sourcePN 
+          (fun b ofs => Mem.perm m b ofs Max Nonempty)
+          (fun b ofs => Mem.perm_dec m b ofs Max Nonempty) n j b2 ofs2.
+
+Lemma sourceN_SomeE: forall n j m b2 ofs2 b1 ofs1, 
+    sourceN n j m b2 ofs2 = Some(b1,ofs1) ->
+    exists delta, 0 <= b1 <= (Z_of_nat n) /\ j b1 = Some(b2,delta) /\ 
+                  Mem.perm m b1 ofs1 Max Nonempty /\ ofs2=ofs1+delta.
+Proof. intros.
+  apply (sourcePN_SomeE
+          (fun b ofs => Mem.perm m b ofs Max Nonempty)
+          (fun b ofs => Mem.perm_dec m b ofs Max Nonempty));
+  auto. 
+Qed. 
+
+Lemma sourceN_NoneE: forall n j m b2 ofs2, 
+    sourceN n j m b2 ofs2 = None -> 
+    forall b1 delta, 0 <= b1 <= (Z_of_nat n) -> j b1 = Some(b2,delta) ->
+                     ~ Mem.perm m b1 (ofs2-delta) Max Nonempty.
+Proof. intros.
+  apply (sourcePN_NoneE
+          (fun b ofs => Mem.perm m b ofs Max Nonempty)
+          (fun b ofs => Mem.perm_dec m b ofs Max Nonempty) n j b2 ofs2);
+  auto. 
+Qed. 
+
+Lemma sourceN_SomeI: forall n j m b2 b1 
+   ofs1 delta (OV:Mem.meminj_no_overlap j m),
+   j b1 = Some(b2,delta) -> Mem.perm m b1 ofs1 Max Nonempty ->
+   (0 <= b1 <= Z_of_nat n) ->
+   sourceN n j m b2 (ofs1+delta) = Some(b1,ofs1).
+Proof. intros. 
+  apply (sourcePN_SomeI
+          (fun b ofs => Mem.perm m b ofs Max Nonempty)
+          (fun b ofs => Mem.perm_dec m b ofs Max Nonempty) n j m);
+  auto. 
+Qed. 
+(*explicit proof:
+unfold sourceN.
+  remember (sourcePN (fun b ofs => Mem.perm m b ofs Max Nonempty)
+          (fun b ofs => Mem.perm_dec m b ofs Max Nonempty) n j b2 (ofs1 + delta)) as src.
+  destruct src; apply eq_sym in Heqsrc. 
+  Focus 2. assert (ZZ:= sourcePN_NoneE _ _ _ _ _ _ Heqsrc _ _ H1 H).
+           exfalso. assert (ofs1 + delta - delta = ofs1). omega.
+                    rewrite H2 in ZZ. apply (ZZ H0).
+  (*Some*) destruct p as [b off].
+       apply sourcePN_SomeE in Heqsrc.
+       destruct Heqsrc as [d [Hd [J [PP X]]]].
+       destruct (eq_block b1 b).
+          subst. rewrite H in J. inv J.
+          assert (ofs1 = off). omega. subst. trivial.
+       destruct (OV _ _ _ _ _ _ _ _ n0 H J H0 PP).
+          exfalso. apply H2; trivial.
+       rewrite X in H2. exfalso. apply H2. trivial.
+Qed.  *)
+
+Definition  source j m (b2:block) (ofs2:Z) : option(block * Z) :=
+   sourceN (Zabs_nat ((Mem.nextblock m) - 1))  j m b2 ofs2.
+
+Lemma source_SomeE: forall j m (b2:block) (ofs2:Z) p, 
+  Some p = source j m b2 ofs2 -> 
+    exists b1, exists delta, exists ofs1, 
+                  p = (b1,ofs1) /\
+                  0 <= b1 < Mem.nextblock m /\ j b1 = Some(b2,delta) /\ 
+                  Mem.perm m b1 ofs1 Max Nonempty /\ ofs2=ofs1+delta.
+Proof. intros. 
+  apply (sourceP_SomeE
+          (fun b ofs => Mem.perm m b ofs Max Nonempty)
+          (fun b ofs => Mem.perm_dec m b ofs Max Nonempty)); 
+  auto. 
+Qed.
+  
+Lemma source_NoneE: forall j m b2 ofs2, 
+    None = source j m b2 ofs2 -> 
+    forall b1 delta, 0 <= b1 < Mem.nextblock m -> j b1 = Some(b2,delta) ->
+                     ~ Mem.perm m b1 (ofs2-delta) Max Nonempty. 
+Proof. intros. 
+  apply (sourceP_NoneE
+          (fun b ofs => Mem.perm m b ofs Max Nonempty)
+          (fun b ofs => Mem.perm_dec m b ofs Max Nonempty) j m b2); 
+  auto. 
+Qed.
+
+Lemma source_SomeI: forall j m b2 b1 ofs1 delta (OV:Mem.meminj_no_overlap j m),
+   j b1 = Some(b2,delta) -> Mem.perm m b1 ofs1 Max Nonempty ->
+   source j m b2 (ofs1+delta) = Some(b1,ofs1).
+Proof. intros. 
+  apply (sourceP_SomeI
+          (fun b ofs => Mem.perm m b ofs Max Nonempty)
+          (fun b ofs => Mem.perm_dec m b ofs Max Nonempty) j m b2); 
+  auto. 
+Qed.
+(*explicit proof
+ unfold source.
+  eapply sourceN_SomeI. apply OV. apply H. apply H0.
+  destruct (VALIDBLOCK _ _ (Mem.perm_valid_block _ _ _ _ _ H0)). 
+  clear H OV. rewrite inj_Zabs_nat.
+  destruct (Zabs_spec (Mem.nextblock m - 1)); destruct H; rewrite H3; omega. 
+Qed.*)
+
+Lemma sourceNone_LOOR: forall j m1 b2 ofs2 (N: None = source j m1 b2 ofs2) m2
+              (Inj12: Mem.inject j m1 m2), loc_out_of_reach j m1 b2 ofs2.
+Proof. intros. intros b1; intros.
+   eapply source_NoneE.
+     apply N. 
+     apply VALIDBLOCK. apply (Mem.valid_block_inject_1 _ _ _ _ _ _ H Inj12).
+     apply H.
+Qed.
+
 
 Lemma mymemvalUnchOnR: forall m1 m2 m3 m3' b ofs 
   (n : ~ Mem.perm m1 b ofs Max Nonempty)
