sepcomp-reserved/RG_interpolants.v
@@ -1,7 +1,16 @@
+Require Import Events.
+Require Import Memory.
+Require Import AST.
+Require Import Coqlib.
+Require Import Values.
+Require Import Maps.
+Require Import Integers.
+Require Import Globalenvs.
 
-
+Require Import sepcomp.mem_lemmas.
+Require Import sepcomp.core_semantics.
 (*CompCert imports*)
-Add LoadPath "../compcert/lib".
+(*Add LoadPath "../compcert/lib".
 Add LoadPath "../compcert/flocq/Appli".
 Add LoadPath "../compcert/flocq/Calc".
 Add LoadPath "../compcert/flocq/Core".
@@ -20,7 +29,7 @@ Require Import compcert.lib.Integers.
 Require Import compcert.common.Globalenvs.
 
 Require Import sepcomp.mem_lemmas.
-Require Import sepcomp.core_semantics.
+Require Import sepcomp.core_semantics.*)
 (*
 Definition reserve_image (*{F1 V1 C1:Type} 
       (Sem: RelyGuaranteeSemantics (Genv.t F1 V1) C1 (list (ident * globdef F1 V1)))*)
@@ -75,12 +84,16 @@ Parameter interpolate_II: forall {F1 V1 C1 F2 V2 C2:Type}
                              (InjIncr: inject_incr (compose_meminj j12 j23) j')
                              (InjSep: inject_separated (compose_meminj j12 j23) j' m1 m3)
                              (WD1: mem_wd m1) (WD1': mem_wd m1') (WD2: mem_wd m2) (WD3: mem_wd m3) (WD3' : mem_wd m3')
-                             st1 (r r': reserve) st2
+                             (r r': reserve) 
                              (Rinc: reserve_incr r r')
                              (Rsep13: reserve_separated r r' j' m1 m3)
-                             (Unch11': rely Sem1 r st1 m1 m1' )
+                              
+                   RELY1 (RELY1_dec: forall b ofs, {RELY1 b ofs} + {~RELY1 b ofs})
+                   (Uniform1: uniform RELY1 j12)
+                             (Unch11': mem_unchanged_on RELY1 m1 m1' ) (*RELY1 is rely Sem1 r st1:  (Unch11': rely Sem1 r st1 m1 m1' )*)
+                             RELY
+                             (Unch33':  mem_unchanged_on RELY m3 m3' )  (*RELY is rely Sem3 (inject_reserve (compose_meminj j12 j23) r) st3 m3 m3')*)                            
 (*                             (Unch33': rely Sem1 (inject_reserve (compose_meminj j12 j23) r) st1 m3 m3')*)
-                             (Unch33': rely Sem3 (inject_reserve (compose_meminj j12 j23) r) st3 m3 m3')
 (*                             (Unch11': mem_unchanged_on (loc_unmapped (compose_meminj j12 j23)) m1 m1')
                              (Unch33': mem_unchanged_on (loc_out_of_reach (compose_meminj j12 j23) m1) m3 m3')*),
                  exists m2', exists j12', exists j23', j'=compose_meminj j12' j23' /\
@@ -89,14 +102,19 @@ Parameter interpolate_II: forall {F1 V1 C1 F2 V2 C2:Type}
                              inject_separated j12 j12' m1 m2 /\ inject_separated j23 j23' m2 m3 /\
                              (mem_wd m2 -> mem_wd m2') /\
                              reserve_separated r r' j12' m1 m2 /\
-                      exists r23, 
-                             rely Sem1 (inject_reserve j12 r) st1 m2 m2' /\
+                      exists r23,  r23 = inject_reserve j12 r /\
+                      exists (RELY2: block -> Z -> Prop),
+                             (forall b1 ofs b2 delta2, j12 b1 = Some(b2,delta2) -> RELY1 b1 ofs -> RELY2 b2 (ofs + delta2)) /\
+                             mem_unchanged_on RELY2 m2 m2' (*  RELY2 should probably be rely Sem2 (inject_reserve j12 r) st2 m2 m2' *)
 (*                             mem_unchanged_on (loc_out_of_reach j12 m1) m2 m2' /\*)
-                             rely Sem2 r23 st2 m2 m2' /\ 
+
+                             (*again? rely Sem2 r23 st2 m2 m2' /\ *)
+
 (*WAS:                             mem_unchanged_on (loc_unmapped j23) m2 m2' /\ *)
 (*WAS:                             rely Sem2 (inject_reserve j23 r23) st2 m3 m3' /\*)
-                             rely Sem3 (inject_reserve j23 r23) st3 m3 m3' /\
-                             r23 = inject_reserve j12 r.
-(*WAS:                             mem_unchanged_on (loc_out_of_reach j23 m2) m3 m3' /\*)                                
+                        (* /\ exists RELY3,
+                             mem_unchanged_on RELY3 m3 m3' *) (*RELY33 should probably be rely Sem3 (inject_reserve j23 r23) st3 m3 m3' /\*)
+
+(*WAS:                             mem_unchanged_on (loc_out_of_reach j23 m2) m3 m3' /\*) .                         
 
 End RGInterpolationAxioms.
